most part of write_preserves_inv

scripts/stack_model.dfy
@@ -3,6 +3,8 @@ include "flat_memory.dfy"
 module stack {
   import opened integers
   import opened flat_memory
+  import Mul
+  import DivMod
 
   function STACK_MAX_BYTES(): (n: nat)
     ensures n % 4 == 0
@@ -19,7 +21,8 @@ module stack {
     ensures sp > STACK_MAX_BYTES()
     ensures ptr_admissible_32(sp)
 
-  function STACK_END(): nat 
+  function STACK_END(): (n: nat)
+    ensures n % 4 == 0
   {
     STACK_START() - STACK_MAX_BYTES()
   }
@@ -145,6 +148,32 @@ module stack {
       }
     }
 
+    lemma fp_decreasing(stack: seq<uint32>, i: nat)
+      requires |stack| == STACK_MAX_WORDS()
+      requires frames_inv(stack)
+      requires i < |fs|
+      ensures forall j: nat | 0 <= j < i :: fs[i].fp <= fs[j].fp
+      ensures forall j: nat | 0 <= j < i :: fs[i].fp + |fs[j].content| * 4 <= fs[j].fp
+    {
+      if i != 0 {
+        // assert fs[i-1].fp <= fs[i].fp;
+        fp_decreasing(stack, i - 1);
+      }
+    }
+
+    lemma sp_as_lower_bound(stack: seq<uint32>, k: nat)
+      requires |stack| == STACK_MAX_WORDS()
+      requires frames_inv(stack)
+      requires k < |fs| - 1
+      ensures sp + |fs[|fs| - 1].content| * 4 + |fs[k].content| * 4  <= fs[k].fp 
+    {
+      var len := |fs| - 1;
+      fp_decreasing(stack, len);
+      assert forall j: nat | 0 <= j < len :: sp + |fs[len].content| * 4 + |fs[j].content| * 4 <= fs[j].fp;
+    }
+
+    // lemma (stack: seq<uint32>, i: nat)
+
     function write(index: nat, value: uint32): frames_t
       requires |fs| >= 1
       requires index < |fs[|fs| - 1].content|
@@ -154,6 +183,103 @@ module stack {
       var new_content := top_f.content[index := value];
       var new_top_f := top_f.(content := new_content);
       this.(fs := fs[last := new_top_f])
+    }
+
+    lemma write_preserves_inv(stack: seq<uint32>,
+      index: nat, value: uint32,
+      new_frames: frames_t)
+      requires |stack| == STACK_MAX_WORDS()
+      requires write.requires(index, value)
+      requires frames_inv(stack)
+      // requires new_frames == write(index, value)
+      // requires new_stack == 
+    {
+      var new_frames := write(index, value);
+      assert in_stack_addr_range(sp);
+
+      var j := ptr_to_stack_index(sp) + index;
+      var new_stack := stack[j := value];
+
+      var last := |new_frames.fs| - 1;
+
+      forall i | 0 <= i < last
+        ensures new_frames.fs[i].next_fp() == new_frames.fs[i + 1].fp
+      {
+        assert fs[i].fp == new_frames.fs[i].fp;
+      }
+
+      forall i | 0 <= i < |new_frames.fs|
+        ensures new_frames.fs[i].frame_inv(new_stack)
+      {
+        var new_f := new_frames.fs[i];
+        var start := ptr_to_stack_index(new_f.next_fp());
+        var end := ptr_to_stack_index(new_f.fp);
+        if i != last {
+          calc == {
+            new_f.content;
+            fs[i].content;
+            {
+              assert fs[i].frame_inv(stack);
+            }
+            stack[start..end];
+            {
+              calc == {
+                j * 4;
+                ((sp - STACK_END()) / 4 + index) * 4;
+                {
+                  Mul.LemmaMulIsDistributiveAuto();
+                }
+                (sp - STACK_END()) / 4 * 4 + index * 4;
+                {
+                  assume (sp - STACK_END()) / 4 * 4 == sp - STACK_END();
+                }
+                sp - STACK_END() + index * 4;
+              }
+
+              calc == {
+                start * 4;
+                (fs[i].fp - 4 * |fs[i].content| - STACK_END()) / 4 * 4;
+                {
+                  assume false;
+                }
+                fs[i].fp - 4 * |fs[i].content| - STACK_END();
+              }
+
+              calc {
+                (j - start) * 4;
+                j * 4 - start * 4;
+                ==
+                sp + index * 4 - fs[i].fp + |fs[i].content| * 4;
+                ==
+                sp + |fs[i].content| * 4 + index * 4 - fs[i].fp ;
+                <=
+                {
+                  sp_as_lower_bound(stack, i);
+                }
+                index * 4 - |fs[last].content| * 4;
+                <
+                0;
+              }
+
+              assert (j - start) * 4 < 0;
+              assert j < start;
+            }
+            new_stack[start..end];
+          }
+        } else {
+          calc == {
+            new_f.content;
+            fs[i].content[index := value];
+            {
+              assert fs[i].frame_inv(stack);
+            }
+            stack[start..end][index := value];
+            stack[start + index := value][start..end];
+            stack[ptr_to_stack_index(sp) + index := value][start..end];
+            stack[j := value][start..end];
+          }
+        }
+      }
     }
   }
 
